Given, $\alpha = \myvec{a\\b\\c}$.
Let,
\begin{align}
\vec{A}=\myvec{\alpha_1&\alpha_2&\alpha_3}\\
\vec{A}\vec{X}=\alpha\\
\myvec{1 & 0 & -1\\0 & 1 & -1\\1 & -2 & 0}\myvec{x_1\\x_2\\x_3} = \myvec{a\\b\\c}
\end{align}
$ \vec{X}=A^{-1}\alpha$ will give solution of the equation.
\begin{align}
\myvec{1 & 0 & -1 & 1 & 0 & 0\\
0 & 1 & -1 & 0 & 1 & 0\\
1 & -2 & 0 & 0 & 0 & 1}\xleftrightarrow[]{R_3\leftarrow R_3-R_1}\\
\myvec{1 & 0 & -1 & 1 & 0 & 0\\
0 & 1 & -1 & 0 & 1 & 0\\
0 & -2 & 1 & -1 & 0 & 1}
\xleftrightarrow[]{R_3\leftarrow R_3+2R_2}\\
\myvec{1 & 0 & -1 & 1 & 0 & 0\\
0 & 1 & -1 & 0 & 1 & 0\\
0 & 0 & -1 & -1 & 2 & 1}\xleftrightarrow[]{R_3\leftarrow R_3/(-1)}\\
\myvec{1 & 0 & -1 & 1 & 0 & 0\\
0 & 1 & -1 & 0 & 1 & 0\\
0 & 0 & 1 & 1 & -2 & -1}\xleftrightarrow{R_1\leftarrow R_1+R_3}\\
\myvec{1 & 0 & 0 & 2 & -2 & -1\\
0 & 1 & -1 & 0 & 1 & 0\\
0 & 0 & 1 & 1 & -2 & -1}\xleftrightarrow{R_2\leftarrow R_2+R_3}\\
\myvec{1 & 0 & 0 & 2 & -2 & -1\\
0 & 1 & 0 & 1 & -1 & -1\\
0 & 0 & 1 & 1 & -2 & -1}
\end{align}
Thus,
\begin{align}
    A^{-1}=\myvec{
    2 &-2&-1\\
    1&-1&-1\\
    1&-2&-1
    }\\
\vec{X} = A^{-1}\alpha=\myvec{2 &-2&-1\\1&-1&-1\\1&-2&-1}
\myvec{a\\b\\c}
\end{align}
Given, $f$ is a linear functional on $R^3$,
\begin{align}
\vec{\alpha} = \alpha_1 x_1 + \alpha_2 x_2 + \alpha_3 x_3\\
\implies f(\alpha) = \vec{X}^T \myvec{f(\alpha_1)\\f(\alpha_2)\\f(\alpha_3)}
\end{align}
Given, $f(\alpha_1)=0$, $f(\alpha_2)=0$ and $f(\alpha_3)\neq 0$.
\begin{align}
 f(\alpha) &= \vec{X}^T \myvec{0\\0\\f(\alpha_3)}\\
\implies f(\alpha) &= \myvec{a\\b\\c}^T\myvec{2 &1&1\\-2&-1&-2 \\-1&-1&-1}\myvec{0\\0\\f(\alpha_3)}\\
f(\alpha)&=\myvec{a\\b\\c}^T\myvec{f(\alpha_3)\\-2f(\alpha_3)\\-f(\alpha_3)}
\end{align}
Hence,
\begin{align}\label{eq:solutions/3/7/1/c/eq1}
f(\alpha)=f(\alpha_3)(a-2b-c)
\end{align}
Given 
$\alpha$=$\myvec{2&3&-1}$
Substituting value of $\alpha$ in equation \eqref{eq:solutions/3/7/1/c/eq1} we have,
\begin{align}
f(\alpha)=-3f(\alpha_3)\neq 0
\end{align}
Hence proved,$f(\alpha)\neq 0$

   
   

