   We start by taking,\begin{align}\vec{f}=\myvec{1\\x\\x^2}\end{align}
   Let's start by proving that $\vec{g}$ is linearly independent.
    \begin{align}
    \vec{g}=\vec{B}\vec{f}
    \end{align}
    where,
    \begin{align}
    \vec{B}=\myvec{1&0&0\\t&1&0\\t^2&2t&1}
    \end{align}
    Now,
    \begin{align}
    \vec{v}^T\vec{g}=0\\
    \implies \vec{v}^T\vec{B}\vec{f}=0
    \end{align}
    Since $\vec{f}$ is linearly independent,
    \begin{align}
     \vec{v}^T\vec{B}=0\\
     \vec{B}^T\vec{v}=0
    \end{align}
   Since $\vec{B}^T$ is an upper triangular matrix with non zero values in principal diagonal  , it is invertible matrix and hence $\vec{v}$ will be zero vector.Now, Finding the inverse of $\vec{B}^T$
   \begin{align}
   \myvec{1&t&t^2&\vrule&1&0&0\\0&1&2t&\vrule&0&1&0\\0&0&1&\vrule&0&0&1}\\
  \xleftrightarrow{R_1=R_1-tR_2} \myvec{1&0&-t^2&\vrule&1&-t&0\\0&1&2t&\vrule&0&1&0\\0&0&1&\vrule&0&0&1}\\
 \xleftrightarrow{R_1=R_1+t^2R_3}  \myvec{1&0&0&\vrule&1&-t&t^2\\0&1&2t&\vrule&0&1&0\\0&0&1&\vrule&0&0&1}\\
   \xleftrightarrow{R_2=R_2-2tR_3} \myvec{1&0&0&\vrule&1&-t&t^2\\0&1&0&\vrule&0&1&-2t\\0&0&1&\vrule&0&0&1}
   \end{align}
   So, 
   \begin{align}
   (\vec{B}^{T})^{-1}=\myvec{1&-t&t^2\\0&1&-2t\\0&0&1}\label{eq:solutions/2/4/7/inverse}
   \end{align}
   Now, to find the coordinates,
  \begin{align}
  f(x)=\vec{w}^T\vec{g}
  \end{align}
  So,
  \begin{align}
  \vec{c}^T\vec{f}=\vec{w}^T\vec{g}\\
\vec{c}^T\vec{f}=\vec{w}^T\vec{B}\vec{f}\\
(\vec{c}^T-\vec{w}^T\vec{B})\vec{f}=0
  \end{align} 
  Since, $\vec{f}$ is linearly independent,
  \begin{align}
  \vec{c}^T-\vec{w}^T\vec{B}=0\\
  \vec{c}^T=\vec{w}^T\vec{B}\\
  \vec{c}^T\vec{B}^{-1}=\vec{w}^T\\
   (\vec{B}^{-1})^T\vec{c}=\vec{w}\label{eq:solutions/2/4/7/final}\end{align}
   Using \eqref{eq:solutions/2/4/7/inverse} in \eqref{eq:solutions/2/4/7/final}
   \begin{align}
 \vec{w}= \myvec{1&-t&t^2\\0&1&-2t\\0&0&1}\myvec{c_0\\c_1\\c_2}
  \end{align} 

