Let,
\begin{align}
\vec{x}, \vec{y} \in \mathbb{R}^2 
\end{align}
Using transformation on $\vec{T}$, 
\begin{align}
\vec{T}(\vec{x}) =\vec{A}\vec{x} \label{eq:solutions/3/1/1/b/1}
\end{align}
From \eqref{eq:solutions/3/1/1/b/0} we get,
\begin{align}
\vec{A}= \myvec{0&1\\1&0}
\end{align}
With $c$ being a scalar,
\begin{align}
\vec{T}(c\vec{x}+\vec{y}) = \myvec{0&1\\1&0}(c\vec{x}+\vec{y})\\
=\myvec{0&1\\1&0}c\vec{x}+\myvec{0&1\\1&0}\vec{y}\\
=\myvec{0&c\\c&0}\vec{x}+\myvec{0&1\\1&0}\vec{y}\\
=c\myvec{0&1\\1&0}\vec{x}+\myvec{0&1\\1&0}\vec{y}\label{eq:solutions/3/1/1/b/2}
\end{align}
From \eqref{eq:solutions/3/1/1/b/2} we can say,
\begin{align}
\vec{T}(c\vec{x}+\vec{y})=c\vec{T}(\vec{x})+\vec{T}(\vec{y})\label{eq:solutions/3/1/1/b/3}
\end{align}
Hence from \eqref{eq:solutions/3/1/1/b/3} we can say $\vec{T}$ is a Linear Transformation from $\mathbb{R}^2$ to $\mathbb{R}^2$ 
