See Table \ref{eq:solutions/6/6/3/table:1}	
%
\onecolumn
\begin{longtable}{|p{4cm}|p{14cm}|}
\hline
\multirow{3}{*}{Given} 
    	& \\
     	&  Let $\vec{x} \in \mathbb{R}^{2}$\\
     	&{\begin{align}\label{eq:solutions/6/6/3/eq1}
     	& \vec{x} = a\myvec{1\\-1} +b\myvec{1\\2}
     	\end{align}}\\
     	& where $\myvec{a\\b}$ is representation of $\vec{x}$ in new basis.\\
\hline
\multirow{3}{*}{To find} 
     	&\\
        &
        {\begin{align}\label{eq:solutions/6/6/3/eq2}
        \vec{E} \brak{\vec{x}} = a\myvec{1\\-1}
        \end{align}}\\
     	
\hline
\multirow{3}{*}{Finding a Projection $\vec{E}$} & \\
       & As, $\myvec{1\\-1},\myvec{1\\2}$ are linearly independent.\\
       &\\
       & Therefore,\{$\myvec{1\\-1},\myvec{1\\2}\}$ is a basis of $\mathbb{R}^{2}$\\
       &\\
       & As $\vec{x} \in \mathbb{R}^{2}$\\
       &{\begin{align}
       \implies \vec{x} = a\myvec{1\\-1} +b\myvec{1\\2}
       \end{align}}\\
       \hline
       &{\begin{align}
       \implies \vec{x} = \myvec{1&1\\-1&2}\myvec{a\\b}
        \end{align}}\\
        &{\begin{align}
        \implies \myvec{a\\b}=\myvec{1&1\\-1&2}^{-1}\vec{x}
        \end{align}}\\
       &
       {\begin{align}
       \implies \myvec{a\\b} = \myvec{\frac{2}{3}&\frac{-1}{3}\\\frac{1}{3}&\frac{1}{3}}\vec{x}
       \end{align}}\\
       & Therefore,\\
       &{\begin{align}\label{eq:solutions/6/6/3/eq3}
          a &=\myvec{\frac{2}{3}&\frac{-1}{3}}\vec{x}
       \end{align}}\\
       
     & Projection of $\vec{x}$ on subspace spanned by $\myvec{1\\-1}$;\\
     &
     {\begin{align}\label{eq:solutions/6/6/3/eq4}
     & \vec{E}\brak{\vec{x}} = a\myvec{1\\-1}
     \end{align}}\\
     & Substituting \eqref{eq:solutions/6/6/3/eq3} in \eqref{eq:solutions/6/6/3/eq4}\\
     &
     {\begin{align}
       \vec{E}\brak{\vec{x}} = \myvec{1\\-1}\myvec{\frac{2}{3}& \frac{-1}{3}}\vec{x}
       \end{align}}\\
       &{\begin{align}
     \vec{E}\brak{\vec{x}} = \myvec{\frac{2}{3}&\frac{-1}{3}\\\frac{-2}{3}&\frac{1}{3}}\vec{x}
      \end{align}}\\
      &{\begin{align}
      \implies{ \vec{E}= \myvec{\frac{2}{3}&\frac{-1}{3}\\\frac{-2}{3}& \frac{1}{3}}}
      \end{align}}\\
       \hline
       \multirow{3}{*}{Verification} & \\
& If $n\times n$ matrix $\vec{E}$ is projection matrix, then\\
	&$\qquad\qquad\qquad \vec{E}^2=\vec{E}$\\
  &{\begin{align}
  \vec{E^{2}} = \myvec{\frac{2}{3}&\frac{-1}{3}\\\frac{-2}{3}& \frac{1}{3}}\myvec{\frac{2}{3}&\frac{-1}{3}\\\frac{-2}{3}& \frac{1}{3}}
  \implies \vec{E}=\vec{E^{2}}=\myvec{\frac{2}{3}&\frac{-1}{3}\\\frac{-2}{3}& \frac{1}{3}}
  \end{align}}\\
  & Hence, Verified.\\
  \hline
\caption{Finding Projection Matrix}
\label{eq:solutions/6/6/3/table:1}	
\end{longtable}
\twocolumn
