Let L be a non  zero linear transformation.
\begin{align}
    f(x)=a_0+a_1(x)+\cdots+a_n(x^n)
\end{align}
\begin{align}\label{eq:solutions/4/2/6/eq1}
L(f)=L(a_0+a_1(x)+\cdots+a_n(x^n)).
\end{align}

Given,L is any  linear functional on f(x).\\
Hence,
\begin{align}
L(f)=L(f.1)=L(f)L(1)
\end{align}
$\implies L(1)\neq 0$.

Similarly,
\begin{align}
L(1)=L(1)L(1)\\
\implies L(1) =1
\end{align}
Similarly, $\forall a \in \vec{F}$.
\begin{align}\label{eq:solutions/4/2/6/eq2}
    L(a)=L(a.1)
    \implies aL(1)=a
\end{align}
Simplifying \eqref{eq:solutions/4/2/6/eq1} we have,
\begin{align}
L(f)=L(a_0)+L(a_1)L(x)+\cdots+L(a_n)L(x^n)
\end{align}
From \eqref{eq:solutions/4/2/6/eq2} we have,$L(x)=t$.
\begin{align}
 L(f)=a_0+a_1L(x)+\cdots a_nL(x)^n\\
 \implies L(f)=a_0+a_1(t)+\cdots a_n(t)^n
\end{align}
Hence proved,$L(f)=f(t)$ .

   
   

