Refer Table \ref{eq:solutions/3/5/13/table:1}.


\begin{table*}[ht!]
\begin{center}
\begin{tabular}{|l|l|}
\hline
\textbf{Given} & \textbf{Derivation} \\[0.5ex]
\hline
\text{$f$, $g$, $h$ are linear functionals of $\vec{V}$} & 
\text{By contradiction, let us assume $f \not= 0$ and $g \not= 0$. For all $\vec{v} \in \vec{V}$}\\
& \parbox{10cm}{\begin{align}
    h(\vec{v}) &= f(\vec{v}) g(\vec{v}) \\
    h(2\vec{v}) &= f(2\vec{v}) g(2\vec{v})\\
    &=2f(\vec{v}) 2g(\vec{v})\\
    &=4f(\vec{v})g(\vec{v}) \label{eq:solutions/3/5/13/eq:eq1}
\end{align}} \\
& Similarly,\\
& \parbox{10cm}{\begin{align}
    h(2\vec{v}) &= 2h(\vec{v}) \\
    &= 2f(\vec{v})g(\vec{v}) \label{eq:solutions/3/5/13/eq:eq2}
\end{align}} \\
& From equation \eqref{eq:solutions/3/5/13/eq:eq1} and \eqref{eq:solutions/3/5/13/eq:eq2},\\
& \parbox{10cm}{\begin{align}
    \implies 4f(\vec{v})g(\vec{v}) = 2f(\vec{v})g(\vec{v})\\
    \implies f(\vec{v}).g(\vec{v})=0 \label{eq:solutions/3/5/13/eq:eq3}
\end{align}}
\\ [0.5ex]
\hline
\text{Choosing Basis} & 
\text{Let $\vec{B}$ be a basis for $\vec{V}$. Let,}\\
& \parbox{10cm}{\begin{align}
    \vec{B_1} &= \{\vec{b} \in \vec{B}\ \vert \ f(\vec{b})=0\}, \\
    \vec{B_2} &= \{\vec{b} \in \vec{B}\ \vert \ g(\vec{b})=0\}
\end{align}} \\
& Since,\\
& \parbox{10cm}{\begin{align}
    f(\vec{b}).g(\vec{b})=0 \quad \forall \vec{b} \in \vec{B}\\
    \implies f(\vec{b})=0 \text{ or } g(\vec{b})=0\\
    \implies \vec{b} \in \vec{B_1} \text{ or } \vec{b} \in \vec{B_2}
\end{align}}
\\ [0.5ex]
\hline
\text{Choosing $\vec{b_1}$ and $\vec{b_2}$ from basis} & 
Let us choose $\vec{b_1} \in \vec{B_1}-\vec{B_2}$ and $\vec{b_2} \in \vec{B_2}-\vec{B_1}$ \\
& $\implies$ $f(\vec{b_2}) \not = 0$ and $g(\vec{b_1}) \not = 0$\\
& \parbox{10cm}{\begin{align}
    f(\vec{b_1}+\vec{b_2}).g(\vec{b_1}+\vec{b_2})= (f(\vec{b_1})+ f(\vec{b_2})).(g(\vec{b_1})+ g(\vec{b_2}))\\
    =f(\vec{b_1}).g(\vec{b_1}) + f(\vec{b_1}).g(\vec{b_2}) +f(\vec{b_2}).g(\vec{b_1}) + f(\vec{b_2}).g(\vec{b_2})\\
    = 0 + 0 + f(\vec{b_2}).g(\vec{b_1}) + 0\\
    = f(\vec{b_2}).g(\vec{b_1}) \not= 0 \label{eq:solutions/3/5/13/eq:eq6}
\end{align}}\\
& Equation \eqref{eq:solutions/3/5/13/eq:eq6} is contradiction to the fact that $f(\vec{v}).g(\vec{v})=0$.\\
& $\implies \boxed{f=0 \text{ or } g=0}$
\\ [0.5ex]
\hline
\end{tabular}
\caption{Expanation}
\label{eq:solutions/3/5/13/table:1}
\end{center}
\end{table*}
