
\begin{align}
trace(\vec{A}\vec{B})= \sum_{i=1}^{n}\vec{(AB)}_{ii}\\
=\sum_{i=1}^{n}\sum_{k=1}^{n}\vec{A}_{ik}\vec{B}_{ki}\\
=\sum_{i=1}^{n}\sum_{k=1}^{n}\vec{B}_{ki}\vec{A}_{ik}\\
=\sum_{i=1}^{n}\vec{(BA)}_{kk}\\
=trace(\vec{B}\vec{A}) \label{eq:solutions/3/5/3/eq:1}
\end{align}
Hence proved trace($\vec{A}\vec{B}$) = trace($\vec{B}\vec{A}$). Let $\vec{A}$ and $\vec{B}$ be similar matrices then $\exists$ $\vec{S}$ such that,
\begin{align}
\vec{A}= \vec{S}^{-1}\vec{B}\vec{S}
\end{align}
Taking trace of $\vec{A}$ we get,
\begin{align}
trace(\vec{A})= trace(\vec{S}^{-1}\vec{B}\vec{S}) =trace(\vec{S}^{-1}(\vec{B}\vec{S})) \label{eq:solutions/3/5/3/eq:2}
\end{align}
Using \eqref{eq:solutions/3/5/3/eq:1} in \eqref{eq:solutions/3/5/3/eq:2}
\begin{align}
trace(\vec{A})= trace(\vec{S}^{-1}\vec{S}\vec{B})\\
=trace((\vec{S}^{-1}\vec{S})\vec{B})\\
=trace(\vec{I}\vec{B})\\
=trace(\vec{B})
\end{align}
Hence Proved
