Lagrange polynomials are given by,
\begin{align}
P_i = \prod_{i\neq j}\frac{x-t_j}{t_i-t_j}\\
P_1 = \frac{(x-3)(x-1)}{(2-3)(2-1)} = -(x-3)(x-1)\\
P_2 = \frac{(x-2)(x-1)}{(3-2)(3-1)} = \frac{1}{2}(x-2)(x-1)\\
P_3 = \frac{(x-2)(x-3)}{(1-2)(1-3)} = \frac{1}{2}(x-2)(x-3)
\end{align}
Now calculating $E_i$,
\begin{align}
E_1 = P_1(\vec{A})=-(\vec{A}-3\vec{I})(\vec{A}-\vec{I})\\=
-\myvec{-1&0&0&0\\0&-1&0&0\\0&0&0&0\\0&0&0&-2}\myvec{1&0&0&0\\0&1&0&0\\0&0&2&0\\0&0&0&0}\\
\implies E_1=\myvec{1&0&0&0\\0&1&0&0\\0&0&0&0\\0&0&0&0}
\end{align}
\begin{align}
E_2 = P_2(\vec{A})=\frac{1}{2}(\vec{A}-2\vec{I})(\vec{A}-\vec{I})\\=
\frac{1}{2}\myvec{0&0&0&0\\0&0&0&0\\0&0&1&0\\0&0&0&-1}\myvec{1&0&0&0\\0&1&0&0\\0&0&2&0\\0&0&0&0}\\
\implies E_2=\myvec{0&0&0&0\\0&0&0&0\\0&0&1&0\\0&0&0&0}
\end{align}
\begin{align}
E_3 = P_3(\vec{A})=\frac{1}{2}(\vec{A}-2\vec{I})(\vec{A}-3\vec{I})\\=
\frac{1}{2}\myvec{0&0&0&0\\0&0&0&0\\0&0&1&0\\0&0&0&-1}\myvec{-1&0&0&0\\0&-1&0&0\\0&0&0&0\\0&0&0&-2}\\
\implies E_3=\myvec{0&0&0&0\\0&0&0&0\\0&0&0&0\\0&0&0&1}
\end{align}
