Given,
\begin{align}
\vec{A}=\myvec{1 & -1 & 1 \\ 2 & 0 & 1 \\ 3 & 0 & 1}	
\end{align}
Take,
\begin{align}
& \vec{E_1}=\myvec{1 & 0 & 0 \\ -2 & 1 & 0 \\ 0 & 0 & 1} \\
& \vec{E_2} = \myvec{1 & 0 & 0 \\0 & 1 &0 \\ -3 & 0&1} \\
& \vec{E_3} = \myvec{1 & 0 & 0 \\0 & \frac{1}{2} &0 \\ 0 & 0&1} \\
& \vec{E_4} = \myvec{1 & 1 & 0 \\0 & 1 &0 \\ 0 & 0&1}
\end{align}
\begin{align}
& \vec{E_5} = \myvec{1 & 0 & 0 \\0 & 1 &0 \\ 0 & -3&1} \\	
& \vec{E_6} = \myvec{1 & 0 & 0 \\0 & 1 &0 \\ 0 & 0& \frac{2}{7}} \\	
& \vec{E_7} = \myvec{1 & 0 & \frac{-1}{2} \\0 & 1 &0 \\ 0 & 0& 1} \\	
& \vec{E_8} = \myvec{1 & 0 & 0 \\0 & 1 &\frac{1}{2} \\ 0 & 0& 1}	
\end{align}
Now, we calculate
\begin{align}
& \vec{E_8E_7E_6E_5E_4E_3E_2E_1}= \myvec{0 & -1 & 1 \\ -1 & 2 & -1 \\ 0 & 3 & -2} 
\end{align}
Hence,
\begin{multline}
\brak{\vec{E_8E_7E_6E_5E_4E_3E_2E_1}}\vec{A} =\\ \myvec{0 & -1 & 1 \\ -1 & 2 & -1 \\ 0 & 3 & -2}\myvec{1 & -1 & 1 \\ 2 & 0 & 1 \\ 3 & 0 & 1} = 
\myvec{1 & 0 & 0 \\ 0 & 1 & 0 \\ 0 & 0 & 1}
\end{multline}
