	we have $\vec{E}$ and it  is idempotent. And we know that the eigen value of idempotent matrix is either 0 or 1.
	When we add the identity matrix in this:
	\begin{align}
	\vec{I} + \vec{E}
	\end{align}
	Then eigen value will be either 1 or 2. Hence $\myvec{\vec{I} + \vec{E}}$ is invertible.
	Since $\vec{E}$ is an idempotent matrix, that is :
	\begin{align}
	\vec{E}^2 = \vec{E} \label{eq:solutions/6/6/9/2.1}
	\intertext{Let,}
	\vec{A} = \vec{I} + \vec{E} \label{eq:solutions/6/6/9/2.3}\\  
	\implies \vec{E} = \vec{A} - \vec{I}\label{eq:solutions/6/6/9/2.4}
	\end{align}
	\begin{align}
	\implies \vec{E}^2 = (\vec{A} - \vec{I})(\vec{A} - \vec{I})= \vec{A}^2 - 2\vec{A} +\vec{I}^2
	\end{align}
	\begin{align}
	\intertext{From \ref{eq:solutions/6/6/9/2.1},}
	\implies  \vec{E} = \vec{A}^2 -2\vec{A} + \vec{I}
	\end{align}
	\begin{align}
	\intertext{Using \eqref{eq:solutions/6/6/9/2.4} we have,}
	\implies \vec{A} - \vec{I} = \vec{A}^2 -2\vec{A} +\vec{I} = \vec{A}^2 -3\vec{A} + 2\vec{I} = 0
	\end{align}
	\begin{align}
	\implies \vec{I} = \frac{ 3\vec{A} - \vec{A}^2}{2}
	\end{align}
	multiplying $\vec{A}^{-1}$ both side,
	\begin{align}
	\vec{A}^{-1} = \frac{3\vec{I}-\vec{A}}{2} = \frac{3\vec{I} - (\vec{I} +\vec{E})}{2}\\
\implies \vec{A^{-1}} = \frac{2\vec{I}- \vec{E}}{2}\\
	\intertext{Using \eqref{eq:solutions/6/6/9/2.3}, we  have,}
(\vec{I} + \vec{E})^{-1} =  \vec{I}- \frac{1}{2}\vec{E} \label{eq:solutions/6/6/9/2.11}
	\end{align}
%
	Let consider a matrix $\vec{E}$ as :
	\begin{align}
	\vec{E} =  \myvec{1 & 0 \\ 0 & 0}\\
	\implies \vec{E}^2 = \myvec{1 & 0 \\ 0 & 0}\myvec{1 & 0 \\ 0 & 0} = \myvec{1 & 0 \\ 0 & 0}\\
\implies \vec{E}^2 = E.\\
\intertext{Now,}
\vec{I}+ \vec{E} = \myvec{1 & 0 \\ 0 & 1} + \myvec{ 1 & 0 \\ 0 & 0}\\
\implies \vec{I} + \vec{E} = \myvec{2 & 0 \\ 0 & 1} = \myvec{2 & 0 \\ 0 &1} \label{eq:solutions/6/6/9/3.8}\\
\end{align}	
Now let find the eigen value of matrix $\myvec{\vec{I} + \vec{E}}$ :
\begin{align}
\implies \myvec{2 - \lambda  & 0 \\ 0  &  1 - \lambda} = 0\\
\implies (2-\lambda)(1 - \lambda) = 0\\
\implies \lambda_1 = 2, \lambda_2 = 1 \label{eq:solutions/6/6/9/3.16}
\end{align}
 
The eigen values of the matrix $(\vec{I} + \vec{E})$ from \eqref{eq:solutions/6/6/9/3.16} are  2 and 1. Since none of the eigen value is zero, hence matrix is invertible.\\
Inverse of the matrix  from \eqref{eq:solutions/6/6/9/2.11} is :
\begin{align}
  \myvec{\vec{I} + \vec{E}}^{-1} =\myvec{1 & 0 \\ 0 & 1} +  \myvec{ -\frac{1}{2} & 0 \\ 0 & 1} \label{eq:solutions/6/6/9/3.19}
\end{align}
	
