See Table     \ref{eq:solutions/6/2/8/tab:my_label}

\begin{table*}[h]
    \centering
    \begin{tabular}{|c|c|}
         \hline
         Invertible & A matrix $\vec{M}$ is invertible if it is non-singular i.e. the null space of $\vec{M}$ contains only \\
         & zero vector.If $\vec{x}$ is a vector such that $\vec{M}\vec{x}=0\implies \vec{x}=0$\\
         \hline
         Proof for 1 & Consider a vecor $\vec{y}$ such that $\brak{\vec{I}-\vec{B}\vec{A}}\vec{y}=0$\\
         & $\brak{\vec{I}-\vec{B}\vec{A}}\vec{y}=0\implies\vec{y}=\vec{BA}\vec{y}$\\
         & $\vec{A}\vec{y}=\vec{ABA}\vec{y}\implies\brak{\vec{I}-\vec{A}\vec{B}}\vec{A}\vec{y}=0$\\
         & since the matrix $\brak{\vec{I}-\vec{A}\vec{B}}$ is invertible,$\vec{A}\vec{y}=0$\\
         & $\vec{y}=\vec{B}\brak{\vec{Ay}}\implies\vec{y}=0$\\
         & Hence the matrix $\brak{\vec{I}-\vec{B}\vec{A}}$ is invertible.\\
         \hline
         Observation & Let $\vec{C}=\brak{\vec{I}-\vec{AB}}^{-1}$,then\\
         & $\brak{\vec{I}-\vec{BA}}\brak{\vec{BCA}}=\vec{BCA}-\vec{BABCA}=\vec{B}\brak{\vec{I}-\vec{AB}}\vec{CA}=\vec{BC^{-1}CA}=\vec{BA}$\\
         & $\vec{\brak{\vec{I}-\vec{BA}}\brak{\vec{BCA}}=\vec{BA}}$\\
         \hline
         Proof for 2 & Let us consider the product $\vec{\brak{I-BA}\brak{BCA+I}}$\\
         & $\vec{\brak{I-BA}\brak{BCA+I}}=\vec{\brak{\vec{I}-\vec{BA}}\brak{\vec{BCA}}}+\brak{\vec{I-BA}}$\\
         & $=\vec{BA+I-BA}=\vec{I}$\\
         & $\brak{\vec{I-BA}}^{-1}=\vec{I+B\brak{I-AB}^{-1}A}$\\
         & Hence proved.\\
         \hline
    \end{tabular}
    \caption{Proof}
    \label{eq:solutions/6/2/8/tab:my_label}
\end{table*}
