 \begin{align}
     A^{2}=\myvec{1&-1&1\\2&0&1\\3&0&1}\myvec{1&-1&1\\2&0&1\\3&0&1}
\end{align}
\begin{align}
     A^{2}=\myvec{2&-1&1\\5&-2&3\\6&-3&4}
 \end{align}
 and
 \begin{align}
   AB=\myvec{1&-1&1\\2&0&1\\3&0&1}\myvec{2&-2\\1&3\\4&4}
\end{align}
\begin{align}
     AB=\myvec{5&-1\\8&0\\10&-2}
 \end{align}
  Now RHS is 
  \begin{align}
     A^{2}B=\myvec{2&-1&1\\5&-2&3\\6&-3&4}\myvec{2&-2\\1&3\\4&4}
 \end{align}
 \begin{align}
    A^{2}B=\myvec{7&-3\\20&-4\\25&-5}
 \end{align}
  Now LHS is 
  \begin{align}
     A(AB)=\myvec{1&-1&1\\2&0&1\\3&0&1}\myvec{5&-1\\8&0\\10&-2}
 \end{align}
 \begin{align}
    A(AB)=\myvec{7&-3\\20&-4\\25&-5}
 \end{align}
 Hence verified.
