See Table \ref{eq:solutions/3/4/9/table:1}.

\begin{table*}[h!]
\begin{center}
\begin{tabular}{|l|l|}
\hline
Assume $[S]_\mathcal{B} = [T]_\mathcal{B'}$ & Assume $\vec{T} = \vec{U}\vec{S}\vec{U}^{-1}$\\[0.5ex]\hline
 & \\
\textbf{Given}&\textbf{Given}\\
 & \\
$\mathbb V$ is a finite dimensional vector space over field $\mathbb F$ & $\mathbb V$ is a finite dimensional vector space over field $\mathbb F$\\ $\vec{S}$ and $\vec{T}$ are linear operators on $\mathbb V$ & $\vec{S}$ and $\vec{T}$ are linear operators on $\mathbb V$\\
$\mathcal{B}$ and $\mathcal{B}'$ are ordered bases for $\mathbb V$ & $\mathcal{B}$ and $\mathcal{B}'$ are ordered bases for $\mathbb V$\\
$[S]_\mathcal{B} = [T]_\mathcal{B}'$ & There is an invertible linear operator $\vec{U}$ on $\mathbb V$\\
 &  such that $\vec{T} = \vec{U}\vec{S}\vec{U}^{-1}$\\ [0.5ex] \hline
  & \\
\textbf{To prove}&\textbf{To prove}\\
 & \\
There is an invertible linear operator $\vec{U}$ on $\mathbb V$ & $[S]_\mathcal{B} = [T]_\mathcal{B}'$\\
such that $\vec{T} = \vec{U}\vec{S}\vec{U}^{-1}$ & \\ [0.5ex] \hline
 & \\
\textbf{Assumptions}&\textbf{Assumptions}\\
 & \\
Let $\vec{U}$ be the operator which carries $\mathcal{B}$ to $\mathcal{B}'$ &
Let $\vec{U}$ be the operator which carries $\mathcal{B}$ to $\mathcal{B}'$\\
$\mathcal{B} = \{\vec{x}_1,\vec{x}_2,\ldots,\vec{x}_n\}$ &
$\mathcal{B} = \{\vec{x}_1,\vec{x}_2,\ldots,\vec{x}_n\}$\\
$\mathcal{B}' = \{\vec{x}_1',\vec{x}_2',\ldots,\vec{x}_n'\}$ &
$\mathcal{B}' = \{\vec{x}_1',\vec{x}_2',\ldots,\vec{x}_n'\}$\\ [0.5ex] \hline
 & \\
\textbf{Proof}&\textbf{Proof}\\
 & \\
For $\vec{v} \in \mathbb V$, expressed as a linear combination &
For $\vec{v} \in \mathbb V$, expressed as a linear combination\\
of the vectors of $\mathcal{B}$ &
of the vectors of $\mathcal{B'}$\\
$\vec{v} = a_1\vec{x}_1 + a_2\vec{x}_2 + \ldots + a_n\vec{x}_n$ &
$\vec{v} = a_1\vec{x}_1' + a_2\vec{x}_2' + \ldots + a_n\vec{x}_n'$\\
 & \\
$\vec{w} = \vec{U}(\vec{v}) = a_1\vec{x}_1' + a_2\vec{x}_2' + \ldots + a_n\vec{x}_n'$ &
$\vec{U}\vec{S}\vec{U}^{-1}(\vec{v}) = \vec{T}(\vec{v})$\\
 & $\quad\quad\quad= \vec{T}(a_1\vec{x}_1' + a_2\vec{x}_2' + \ldots + a_n\vec{x}_n')$\\
$\because [S]_\mathcal{B} = [T]_\mathcal{B}'$ &
$\quad\quad\quad= c_1\vec{x}_1' + c_2\vec{x}_2' + \ldots + c_n\vec{x}_n'$\\
$\vec{S}(\vec{v}) = c_1\vec{x_1} + c_2\vec{x}_2 + \ldots + c_n\vec{x}_n\quad\text{and}$ & \\
$\vec{T}(\vec{w}) = c_1\vec{x}_1' + c_2\vec{x}_2' + \ldots + c_n\vec{x}_n'$ &
But we know that\\
 & $\vec{U}\vec{S}\vec{U}^{-1}(\vec{v}) = \vec{U}\vec{S}\vec{U}^{-1}(a_1\vec{x}_1' + a_2\vec{x}_2' + \ldots + a_n\vec{x}_n')$\\
$\vec{U}^{-1}\vec{T}\vec{U}(\vec{v})$ &
$\quad\quad\quad\quad= \vec{U}\vec{S}(a_1\vec{x}_1+a_2\vec{x}_2+\ldots+a_n\vec{x}_n)$\\
$=\vec{U}^{-1}\vec{T}(\vec{w})$ & \\
$=\vec{U}^{-1}(c_1\vec{x}_1' + c_2\vec{x}_2' + \ldots + c_n\vec{x}_n')$ &
So, $\vec{S}$ in basis $\mathcal{B}$ has the same entries as $\vec{T}$ in basis $\mathcal{B}'$\\
$= c_1\vec{x}_1 + c_2\vec{x}_2 + \ldots + c_n\vec{x}_n$ &
$\therefore [S]_\mathcal{B} = [T]_\mathcal{B'}$\\
$=\vec{S}(\vec{v})$ & \\
 & \\
$\implies\vec{U}^{-1}\vec{T}\vec{U} = \vec{S}$ & \\
$\implies \vec{T} = \vec{U}\vec{S}\vec{U}^{-1}$ & \\[0.5ex] \hline
\end{tabular}
\caption{}
\label{eq:solutions/3/4/9/table:1}
\end{center}
\end{table*}
