Given matrices $\vec{A}$,$\vec{B}$,$\vec{C}$,$\vec{D}$ commute.

Let $\vec{P}$ be an invertible matrix that can simultaneously diagonalize matrices $\vec{A}$,$\vec{B}$,$\vec{C}$,$\vec{D}$ as below
\begin{align}
    \vec{A}=\vec{P}\vec{\Lambda_a}\vec{P}^{-1}\label{eq:solutions/6/5/4/A}\\
    \vec{B}=\vec{P}\vec{\Lambda_b}\vec{P}^{-1}\label{eq:solutions/6/5/4/B}\\
    \vec{C}=\vec{P}\vec{\Lambda_c}\vec{P}^{-1}\label{eq:solutions/6/5/4/C}\\
    \vec{D}=\vec{P}\vec{\Lambda_d}\vec{P}^{-1}\label{eq:solutions/6/5/4/D}
\end{align}
where $\vec{\Lambda_a}$,$\vec{\Lambda_b}$,$\vec{\Lambda_c}$,$\vec{\Lambda_d}$ are diagonal matrices whose diagonal values are eigenvalues of matrices $\vec{A}$,$\vec{B}$,$\vec{C}$,$\vec{D}$ respectively and matrix $\vec{P}$ is formed by n-linearly independent eigen vectors.

Now \eqref{eq:solutions/6/5/4/E} can be written as
\begin{align}
    \vec{E}=\myvec{\vec{P}\vec{\Lambda_a}\vec{P}^{-1} & \vec{P}\vec{\Lambda_b}\vec{P}^{-1}\\\vec{P}\vec{\Lambda_c}\vec{P}^{-1} & \vec{P}\vec{\Lambda_d}\vec{P}^{-1}}
\end{align}
Using block matrix multiplication, we get
\begin{align}
    \implies&\vec{E}=\myvec{\vec{P} & \vec{0}\\\vec{0} & \vec{P}}\myvec{\vec{\Lambda_a} & \vec{\Lambda_b}\\\vec{\Lambda_c} & \vec{\Lambda_d}}\myvec{\vec{P}^{-1} & \vec{0}\\\vec{0} & \vec{P}^{-1}}\\
    \implies&\vec{E}=\vec{M}\vec{D}\vec{M}^{-1}\label{eq:solutions/6/5/4/Edec}
\end{align}
where
\begin{align}
    \vec{M}=\myvec{\vec{P} & \vec{0}\\\vec{0} & \vec{P}}\\
    \vec{D}=\myvec{\vec{\Lambda_a} & \vec{\Lambda_b}\\\vec{\Lambda_c} & \vec{\Lambda_d}}
\end{align}
Now we will calculate $\det(\vec{E})$,
\begin{align}
    &\mydet{\vec{E}}=\mydet{\vec{M}\vec{D}\vec{M}^{-1}}\\
    \implies&\mydet{\vec{E}}=\mydet{\vec{M}}\mydet{\vec{D}}\mydet{\vec{M}^{-1}}\\
    \implies&\mydet{\vec{E}}=\mydet{\vec{M}}\mydet{\vec{D}}\mydet{\vec{M}}^{-1}\\
    \implies&\mydet{\vec{E}}=\mydet{\vec{D}}\label{eq:solutions/6/5/4/EeqD}\\
    \implies&\mydet{\vec{E}}=\mydet{\vec{\Lambda_a} & \vec{\Lambda_b}\\\vec{\Lambda_c} & \vec{\Lambda_d}}\\
    &=\mydet{\lambda_{1a}&0&\dots&0&\lambda_{1b}&0&\dots&0\\0&\lambda_{2a}&\dots&0&0&\lambda_{2b}&\dots&0\\\vdots&\vdots&\dots&\vdots&\vdots&\vdots&\dots&\vdots\\0&0&\dots&\lambda_{na}&0&0&\dots&\lambda_{nb}\\\lambda_{1c}&0&\dots&0&\lambda_{1d}&0&\dots&0\\0&\lambda_{2c}&\dots&0&0&\lambda_{2d}&\dots&0\\\vdots&\vdots&\dots&\vdots&\vdots&\vdots&\dots&\vdots\\0&0&\dots&\lambda_{nc}&0&0&\dots&\lambda_{nd}}
\end{align}
Using row reduction,
\begin{multline}
    \xleftrightarrow[]{R_{n+1}=R_{n+1}-\frac{\lambda_{1c}}{\lambda_{1a}}R_1}\\
    \mydet{\lambda_{1a}&0&\dots&0&\lambda_{1b}&0&\dots&0\\0&\lambda_{2a}&\dots&0&0&\lambda_{2b}&\dots&0\\\vdots&\vdots&\dots&\vdots&\vdots&\vdots&\dots&\vdots\\0&0&\dots&\lambda_{na}&0&0&\dots&\lambda_{nb}\\0&0&\dots&0&\lambda_{1d}-\frac{\lambda_{1c}\lambda_{1b}}{\lambda_{1a}}&0&\dots&0\\0&\lambda_{2c}&\dots&0&0&\lambda_{2d}&\dots&0\\\vdots&\vdots&\dots&\vdots&\vdots&\vdots&\dots&\vdots\\0&0&\dots&\lambda_{nc}&0&0&\dots&\lambda_{nd}}
\end{multline}
similarly doing elementary row operations for rows $R_{n+2}$ to $R_{2n}$, we get

\begin{multline}
    \mydet{\vec{E}}=\\\mydet{\lambda_{1a}&\dots&0&\lambda_{1b}&\dots&0\\\vdots&\dots&\vdots&\vdots&\dots&\vdots\\0&\dots&\lambda_{na}&0&\dots&\lambda_{nb}\\0&\dots&0&\lambda_{1d}-\frac{\lambda_{1c}\lambda_{1b}}{\lambda_{1a}}&\dots&0\\\vdots&\dots&\vdots&\vdots&\dots&\vdots\\0&\dots&0&0&\dots&\lambda_{nd}-\frac{\lambda_{nc}\lambda_{nb}}{\lambda_{na}}}
\end{multline}
Since it is upper triangular matrix, then $\mydet{\vec{E}}$ will be multiplication of diagonal elements.
\begin{multline}
    \implies\mydet{\vec{E}}=\lambda_{1a}\lambda_{2a}\dots\lambda_{na}\\\times\left(\lambda_{1d}-\frac{\lambda_{1c}\lambda_{1b}}{\lambda_{1a}}\right)\dots\left(\lambda_{nd}-\frac{\lambda_{nc}\lambda_{nb}}{\lambda_{na}}\right)
\end{multline}
\begin{multline}
    \implies\mydet{\vec{E}}=(\lambda_{1a}\lambda_{1d}-\lambda_{1c}\lambda_{1b})\\\times(\lambda_{2a}\lambda_{2d}-\lambda_{2c}\lambda_{2b})\dots(\lambda_{na}\lambda_{nd}-\lambda_{nc}\lambda_{nb})\label{eq:solutions/6/5/4/detE}
\end{multline}

Now we will calculate $\det(\vec{A}\vec{D}-\vec{B}\vec{C})$ by substituting \eqref{eq:solutions/6/5/4/A},\eqref{eq:solutions/6/5/4/B},\eqref{eq:solutions/6/5/4/C},\eqref{eq:solutions/6/5/4/D}
\begin{align}
    \mydet{\vec{A}\vec{D}-\vec{B}\vec{C}}&=\mydet{\vec{P}\vec{\Lambda_a}\vec{P}^{-1}\vec{P}\vec{\Lambda_d}\vec{P}^{-1}-\vec{P}\vec{\Lambda_b}\vec{P}^{-1}\vec{P}\vec{\Lambda_c}\vec{P}^{-1}}\\
    &=\mydet{\vec{P}\vec{\Lambda_a}\vec{\Lambda_d}\vec{P}^{-1}-\vec{P}\vec{\Lambda_b}\vec{\Lambda_c}\vec{P}^{-1}}\\
    &=\mydet{\vec{P}(\vec{\Lambda_a}\vec{\Lambda_d}-\vec{\Lambda_b}\vec{\Lambda_c})\vec{P}^{-1}}\\
    &=\mydet{\vec{P}}\mydet{\vec{\Lambda_a}\vec{\Lambda_d}-\vec{\Lambda_b}\vec{\Lambda_c}}\mydet{\vec{P}^{-1}}\\
    &=\mydet{\vec{P}}\mydet{\vec{P}}^{-1}\mydet{\vec{\Lambda_a}\vec{\Lambda_d}-\vec{\Lambda_b}\vec{\Lambda_c}}\\
    \mydet{\vec{A}\vec{D}-\vec{B}\vec{C}}&=\mydet{\vec{\Lambda_a}\vec{\Lambda_d}-\vec{\Lambda_b}\vec{\Lambda_c}}\label{eq:solutions/6/5/4/adbc1}
\end{align}

Since $\vec{\Lambda_a}$,$\vec{\Lambda_b}$,$\vec{\Lambda_c}$,$\vec{\Lambda_d}$ are diagonal matrices, we get
\begin{align}
    \vec{\Lambda_a}\vec{\Lambda_d}=\myvec{\lambda_{1a}\lambda_{1d}&0&\dots&0\\0&\lambda_{2a}\lambda_{2d}&\dots&0\\\vdots&\vdots&\dots&\vdots\\0&0&\dots&\lambda_{na}\lambda_{nd}}\label{eq:solutions/6/5/4/lald}\\
    \vec{\Lambda_b}\vec{\Lambda_c}=\myvec{\lambda_{1b}\lambda_{1c}&0&\dots&0\\0&\lambda_{2b}\lambda_{2c}&\dots&0\\\vdots&\vdots&\dots&\vdots\\0&0&\dots&\lambda_{nb}\lambda_{nc}}\label{eq:solutions/6/5/4/lblc}\\
\end{align}

Substitute \eqref{eq:solutions/6/5/4/lald} and \eqref{eq:solutions/6/5/4/lblc} in \eqref{eq:solutions/6/5/4/adbc1}, we get
\begin{multline}
    \mydet{\vec{A}\vec{D}-\vec{B}\vec{C}}=\\\mydet{\lambda_{1a}\lambda_{1d}-\lambda_{1b}\lambda_{1c}&\dots&0\\0&\dots&0\\\vdots&\dots&\vdots\\0&\dots&\lambda_{na}\lambda_{nd}-\lambda_{nb}\lambda_{nc}}
\end{multline}
\begin{multline}
    \implies\mydet{\vec{A}\vec{D}-\vec{B}\vec{C}}=(\lambda_{1a}\lambda_{1d}-\lambda_{1b}\lambda_{1c})\\\times(\lambda_{2a}\lambda_{2d}-\lambda_{2b}\lambda_{2c})\dots(\lambda_{na}\lambda_{nd}-\lambda_{nb}\lambda_{nc})\label{eq:solutions/6/5/4/adbcfin}
\end{multline}

Comparing \eqref{eq:solutions/6/5/4/detE} and \eqref{eq:solutions/6/5/4/adbcfin} we can say that
\begin{align}
    \mydet{\vec{E}}=\mydet{\vec{A}\vec{D}-\vec{B}\vec{C}}
\end{align}
Hence proved.
\\
{\em Example: }
Let us consider below matrices $\vec{A}$,$\vec{B}$,$\vec{C}$,$\vec{D}$ be $n\times n$ complex matrices which commute.
\begin{align}
    \vec{A}=\myvec{1-i&-2\\3&-1-i}\label{eq:solutions/6/5/4/exa}\\
    \vec{B}=\myvec{3-3i&-6\\9&-3-3i}\label{eq:solutions/6/5/4/exb}\\
    \vec{C}=\myvec{7-7i&-14\\21&-7-7i}\label{eq:solutions/6/5/4/exc}\\
    \vec{D}=\myvec{-2+2i&4\\-6&2+2i}\label{eq:solutions/6/5/4/exd}
\end{align}
Lets find eigenvalues of matrix $\vec{A}$
\begin{align}
    &\mydet{\vec{A}-\lambda\vec{I}}=0\\
    \implies&\mydet{1-i-\lambda&-2\\3&-1-i-\lambda}=0\\
    \implies&\lambda^2+2\lambda i+4=0\\
    \implies&\lambda_{1a}=-(1+\sqrt{5})i\quad\lambda_{2a}=(-1+\sqrt{5})i\label{eq:solutions/6/5/4/eiga}
\end{align}
\eqref{eq:solutions/6/5/4/eiga} are eigenvalues of matrix $\vec{A}$.

The eigenvectors of matrix $\vec{A}$ are
\begin{align}
    \vec{v_1}=\myvec{\frac{-1+\sqrt{5}i}{3}\\1}\quad\vec{v_2}=\myvec{\frac{-1-\sqrt{5}i}{3}\\1}
\end{align}
Since matrices $\vec{A}$,$\vec{B}$,$\vec{C}$,$\vec{D}$ commute, from \eqref{eq:solutions/6/5/4/exa}, \eqref{eq:solutions/6/5/4/exb}, \eqref{eq:solutions/6/5/4/exc}, \eqref{eq:solutions/6/5/4/exd} we can say that
\begin{align}
    \vec{B}&=3\vec{A}\\
    \vec{C}&=7\vec{A}\\
    \vec{D}&=-2\vec{A}
\end{align}

Then the eigenvalues of matrices $\vec{B}$,$\vec{C}$,$\vec{D}$ are
\begin{align}
    \lambda_{1b}=-3(1+\sqrt{5})i\quad\lambda_{2b}=3(-1+\sqrt{5})i\label{eq:solutions/6/5/4/eigb}\\
    \lambda_{1c}=-7(1+\sqrt{5})i\quad\lambda_{2c}=7(-1+\sqrt{5})i\label{eq:solutions/6/5/4/eigc}\\
    \lambda_{1d}=2(1+\sqrt{5}+1)i\quad\lambda_{2d}=-2(-1+\sqrt{5})i\label{eq:solutions/6/5/4/eigd}
\end{align}
But the eigenvectors of matrices $\vec{B}$,$\vec{C}$,$\vec{D}$ are same as of matrix $\vec{A}$.\\
The eigenvalue decomposition of matrices $\vec{A}$,$\vec{B}$,$\vec{C}$,$\vec{D}$ is done as in \eqref{eq:solutions/6/5/4/A}, \eqref{eq:solutions/6/5/4/B}, \eqref{eq:solutions/6/5/4/C}, \eqref{eq:solutions/6/5/4/D}. Here eigenvector matrix $\vec{P}$ and $\vec{\Lambda_a}$,$\vec{\Lambda_b}$,$\vec{\Lambda_c}$,$\vec{\Lambda_d}$ are
\begin{align}
    \vec{P}=\myvec{\frac{-1+\sqrt{5}i}{3}&\frac{-1-\sqrt{5}i}{3}\\1&1}\\
    \vec{\Lambda_a}=\myvec{mi&0\\0&ni}\label{eq:solutions/6/5/4/exla}\\
    \vec{\Lambda_b}=\myvec{3mi&0\\0&3ni}\label{eq:solutions/6/5/4/exlb}\\
    \vec{\Lambda_c}=\myvec{7mi&0\\0&7ni}\label{eq:solutions/6/5/4/exlc}\\
    \vec{\Lambda_d}=\myvec{-2mi&0\\0&-2ni}\label{eq:solutions/6/5/4/exld}
\end{align}
where
\begin{align}
    m=-(1+\sqrt{5})\quad n=(-1+\sqrt{5})\label{eq:solutions/6/5/4/mn}
\end{align}
From \eqref{eq:solutions/6/5/4/Edec}, we got
\begin{align}
    \vec{E}=\vec{M}\vec{D}\vec{M}^{-1}
\end{align}
where
\begin{align}
    \vec{M}&=\myvec{\vec{P} & \vec{0}\\\vec{0} & \vec{P}}\\
    &=\myvec{\frac{-1+\sqrt{5}i}{3}&\frac{-1-\sqrt{5}i}{3}&0&0\\1&1&0&0\\0&0&\frac{-1+\sqrt{5}i}{3}&\frac{-1-\sqrt{5}i}{3}\\0&0&1&1}
\end{align}
\begin{multline}
    \vec{D}=\myvec{\vec{\Lambda_a} & \vec{\Lambda_b}\\\vec{\Lambda_c} & \vec{\Lambda_d}}\\
    =\myvec{mi&0&3mi&0\\0&ni&0&3ni\\7mi&0&-2mi&0\\0&7ni&0&-2ni}
\end{multline}
Now we will calculate $\det(E)$, from \eqref{eq:solutions/6/5/4/EeqD} we got
\begin{align}
    \mydet{\vec{E}}&=\mydet{\vec{D}}\\
    &=\mydet{mi&0&3mi&0\\0&ni&0&3ni\\7mi&0&-2mi&0\\0&7ni&0&-2ni}
\end{align}
Using row reduction technique,
\begin{align}
    \mydet{mi&0&3mi&0\\0&ni&0&3ni\\7mi&0&-2mi&0\\0&7ni&0&-2ni}\\
    \xleftrightarrow[]{R_3\leftarrow R_3-7R_1}\mydet{mi&0&3mi&0\\0&ni&0&3ni\\0&0&-23mi&0\\0&7ni&0&-2ni}\\
    \xleftrightarrow[]{R_4\leftarrow R_4-7R_2}\mydet{mi&0&3mi&0\\0&ni&0&3ni\\0&0&-23mi&0\\0&0&0&-23ni}
\end{align}
Now
\begin{align}
    \mydet{\vec{E}}=\mydet{mi&0&3mi&0\\0&ni&0&3ni\\0&0&-23mi&0\\0&0&0&-23ni}\\
    \implies\mydet{\vec{E}}=529m^2n^2\label{eq:solutions/6/5/4/exdet1}
\end{align}
Substitute \eqref{eq:solutions/6/5/4/mn} in \eqref{eq:solutions/6/5/4/exdet1}, we get
\begin{align}
    \mydet{\vec{E}}=529(1+\sqrt{5})^2(-1+\sqrt{5})^2=8464\label{eq:solutions/6/5/4/exdetfin}
\end{align}
Now we will calculate $\det(\vec{A}\vec{D}-\vec{B}\vec{C})$, from \eqref{eq:solutions/6/5/4/adbc1} we got
\begin{align}
    \mydet{\vec{A}\vec{D}-\vec{B}\vec{C}}&=\mydet{\vec{\Lambda_a}\vec{\Lambda_d}-\vec{\Lambda_b}\vec{\Lambda_c}}\label{eq:solutions/6/5/4/exadbc1}
\end{align}
Using \eqref{eq:solutions/6/5/4/exla}, \eqref{eq:solutions/6/5/4/exlb}, \eqref{eq:solutions/6/5/4/exlc}, \eqref{eq:solutions/6/5/4/exld} we get
\begin{align}
    \vec{\Lambda_a}\vec{\Lambda_d}&=\myvec{mi&0\\0&ni}\myvec{-2mi&0\\0&-2ni}\\
    \implies\vec{\Lambda_a}\vec{\Lambda_d}&=\myvec{2m^2&0\\0&2n^2}\label{eq:solutions/6/5/4/exlald}\\
    \vec{\Lambda_b}\vec{\Lambda_c}&=\myvec{3mi&0\\0&3ni}\myvec{7mi&0\\0&7ni}\\
    \implies\vec{\Lambda_b}\vec{\Lambda_c}&=\myvec{-21m^2&0\\0&-21n^2}\label{eq:solutions/6/5/4/exlblc}
\end{align}
Substitute \eqref{eq:solutions/6/5/4/exlald} and \eqref{eq:solutions/6/5/4/exlblc} in \eqref{eq:solutions/6/5/4/exadbc1}, we get
\begin{align}
    \mydet{\vec{A}\vec{D}-\vec{B}\vec{C}}&=\mydet{\myvec{2m^2&0\\0&2n^2}-\myvec{-21m^2&0\\0&-21n^2}}\\
    &=\mydet{23m^2&0\\0&23n^2}\\
    &=529m^2n^2
%\label{eq:solutions/6/5/4/exadbc1}
\end{align}
Substitute \eqref{eq:solutions/6/5/4/mn} in \eqref{eq:solutions/6/5/4/exadbc1}, we get
\begin{multline}
    \mydet{\vec{A}\vec{D}-\vec{B}\vec{C}}=529(1+\sqrt{5})^2(-1+\sqrt{5})^2\\=8464\label{eq:solutions/6/5/4/exadbcfin}
\end{multline}
Comparing \eqref{eq:solutions/6/5/4/exdetfin} and \eqref{eq:solutions/6/5/4/exadbcfin}, we get
\begin{align}
    \mydet{\vec{E}}=\mydet{\vec{A}\vec{D}-\vec{B}\vec{C}}
\end{align}
