We have to find,
\begin{align}
 tr\brak{\vec{C}} = C_{11}+C_{22} = tr\brak{\vec{AB}-\vec{BA}}\\
 \implies  tr\brak{\vec{C}} = tr\brak{\vec{AB}}-tr\brak{\vec{BA}}\label{eq:solutions/1/3/8/s}
\end{align}
We know that,
\begin{align}
tr\brak{\vec{AB}} = \sum_{i=1}^2(\vec{AB})_{ii}\\
\implies \sum_{i=1}^2\sum_{j=1}^2a_{ij}b_{ji}\\
\implies \sum_{j=1}^2\sum_{i=1}^2b_{ji}a_{ij}\\
\implies tr\brak{\vec{AB}} = \sum_{j=1}^2\vec{BA}_{jj}\\
\implies tr\brak{\vec{AB}} = tr\brak{\vec{BA}}
\label{eq:solutions/1/3/8/t}
\end{align}
Substituting equation \eqref{eq:solutions/1/3/8/t} to \eqref{eq:solutions/1/3/8/s} we get
\begin{align}
\implies  tr\brak{\vec{C}} = tr\brak{\vec{AB}}-tr\brak{\vec{BA}} = 0
\end{align}

